refactoring semChecker

src/SemChecker.v
@@ -1,8 +1,7 @@
-Require Import ssreflect ssrbool eqtype.
+Require Import ssreflect ssrbool ssrnat eqtype.
 Require Import Show Sets GenLow GenHigh RoseTrees Checker Arbitrary.
 
 Import GenLow GenHigh.
-
 
 Definition resultSuccessful (r : Result) : bool :=
   match r with
@@ -19,23 +18,36 @@ Definition successful qp :=
 (* CH: The forall+implications in semCheckerSize and semChecker_def2
    are just set inclusions ... wouldn't it be more convenient to treat
    them that way? *)
+(* ZP: Yes, they are now *) 
 
 (* Maps a Checker to a Prop *)
+
 (* begin semCheckerSize *)
 Definition semCheckerSize (c : Checker) (s : nat): Prop :=
-  forall res, res \in semGenSize c s -> successful res = true.
+  successful @: semGenSize c s \subset [set true].
 (* end semCheckerSize *)
-(* begin semChecker *) 
+
+(* ZP: Do we want to define semChecker in terms of semCheckerSize? *)
+
+(* begin semChecker *)
 Definition semChecker (c : Checker) : Prop := forall s, semCheckerSize c s.
 (* end semChecker *)
-(* another characterization of semChecker *)
-Lemma semChecker_def2 c :
-  semChecker c <-> (forall qp, semGen c qp -> successful qp = true).
-Proof.
-  rewrite /semChecker /semCheckerSize /semGen. split; intro H.
-  - intros. destruct H0 as [s H0]. eapply (H s). tauto.
-  - intros. apply H. exists s. by split.
-Qed.
+
+(* Maps a Checkable to a Prop i.e. gives an equivalent proposition to the
+   property under test *)
+
+(* begin semCheckableSize *)
+Definition semCheckableSize {A} `{Checkable A} (a : A) (s : nat) : Prop :=
+  semCheckerSize (checker a) s.
+(* end semCheckableSize *)
+
+(* begin semCheckable *)
+Definition semCheckable {A} `{Checkable A} (a : A) : Prop := semChecker (checker a).
+(* end semCheckable *)
+
+(* TODO : Move these to the set library *)
+
+(* Begin Lemmas for Maxime's library *)
 
 Lemma one_more_for_maximes_library a b x (f : a -> b) (A : set a) :
   x \in A -> f x \in (f @: A).
@@ -43,242 +55,11 @@ Proof.
   intros. unfold imset. exists x. split; by [].
 Qed.
 
-(* CH: This is the definition of Checker I would like to use *)
-Lemma semChecker_def3 c :
-  semChecker c <-> (successful @: semGen c \subset [set true]).
-Proof.
-  rewrite semChecker_def2. split; intro H.
-(*  CH: why can't I rewrite with semFmap directly? See tentative instances below *)
-  - intros b H'. unfold imset, bigcup in H'.
-    destruct H' as [qp [H1 H2]]. apply H in H1. by rewrite H1 in H2.
-  - intros. unfold set_incl in H. specialize (H (successful qp)).
-    unfold set1 in H. symmetry. apply H. clear H.
-    by apply one_more_for_maximes_library.
-Qed.
-
-(*
-Lemma semCheckerSized_def3 c :
-  semCheckerSized c s <-> (successful @: semGenSized c s \subset [set true]).
-*)
-
-(* Maps a Checkable to a Prop i.e. gives an equivalent proposition to the
-   property under test *)
-(* begin semCheckable *)
-Definition semCheckable {A} `{Checkable A} (a : A) : Prop := semChecker (checker a).
-(* end semCheckable *)
-(* begin semCheckableSize *)
-Definition semCheckableSize {A} `{Checkable A} (a : A) (s : nat) : Prop :=
-  semCheckerSize (checker a) s.
-(* end semCheckableSize *)
-
-Lemma mapTotalResult_id {C} `{Checkable C} (f : Result -> Result) (c : C) s :
-    (forall res, resultSuccessful res = resultSuccessful (f res)) ->
-    (semCheckerSize (mapTotalResult f c) s <-> semCheckableSize c s).
-Proof.
-  move=> eq_res.
-  rewrite /mapTotalResult /mapRoseResult /mapProp.
-  split=> [check_map [[res l]] sem_checker|] /=.
-  rewrite eq_res.
-  pose qp := {| unProp := MkRose res l |}.
-  pose qp' := {| unProp := fmapRose f (MkRose res l) |}.
-  by apply/(check_map qp')/semFmapSize; exists qp.
-  move=> sem_p qp /semFmapSize [[[res l]] [? <-]] /=; rewrite -eq_res.
-    by pose qp' := {| unProp := MkRose res l |}; apply: (sem_p qp').
-Qed.
-
-Lemma semCallback_id {C} `{Checkable C} (cb : Callback) (c : C) (s : nat) :
-    semCheckerSize (callback cb c) s <-> semCheckableSize c s.
-Proof.
-  rewrite /callback.
-  split; move => H'.
-  - apply mapTotalResult_id in H' => //;
-    by move => [? ? ? ? ? ?].
-  - apply mapTotalResult_id => //;
-    by move => [? ? ? ? ? ?].
-Qed.
-
-Lemma semWhenFail_id {C} `{Checkable C} (str : String.string) (c : C) s :
-    semCheckerSize (whenFail str c) s <-> semCheckableSize c s.
-Proof.
-  by rewrite /whenFail semCallback_id.
-Qed.
-
-Lemma semPrintTestCase_id {C} `{Checkable C} (str : String.string) (c : C) s :
-    semCheckerSize (printTestCase str c) s <-> semCheckableSize c s.
-Proof.
-  by rewrite /printTestCase semCallback_id.
-Qed.
-
-(* TODO : This proof needs refactoring! *)
-Lemma semShrinking_id {C A} {HCheck : Checkable C}
-         (sh : A -> list A) (x : A) (pf : A -> C) (s : nat) :
-    semCheckerSize (shrinking sh x pf) s <->
-    semCheckableSize (pf x) s.
-Proof.
-  unfold semCheckableSize, shrinking, semCheckerSize, semGenSize.
-  split.
-  - unfold props. generalize 1000.
-    case => [| n] H qp [seed Hgen]; subst.
-    + apply H. apply semFmapSize. eexists.
-      split. apply semPromoteSize.
-      exists seed. simpl. reflexivity.
-      simpl.
-      by destruct ((run (checker (pf x)) s seed)) as [[res [l]]] => /=.
-    + suff :
-        successful
-          (run
-             (fmap
-                (fun x0 => {| unProp := joinRose (fmapRose unProp x0) |})
-                (promote (@props' _ _ HCheck (S n) pf sh x))) s seed).
-      remember
-        (run
-           (fmap
-              (fun x0 : Rose QProp =>
-                 {| unProp := joinRose (fmapRose unProp x0) |})
-              (promote (props' (S n) pf sh x))) s seed) as b.
-      setoid_rewrite runFmap in Heqb. rewrite {}Heqb.
-      rewrite runPromote. simpl.
-      by destruct ((run (checker (pf x)) s seed)) as [[res [l]]] => /=.
-      apply H.
-      apply semFmapSize. eexists. split => /=.
-      apply semPromoteSize.  exists seed. reflexivity.
-      simpl. rewrite runFmap.
-      remember ((run
-                     (promote
-                        (MkRose (checker (pf x))
-                           {| force := List.map (props' n pf sh) (sh x) |}))
-                     s seed)) as b.
-      symmetry in Heqb. setoid_rewrite runPromote in Heqb. by rewrite -Heqb.
-  - unfold props, semGenSize. generalize 1000.
-    move => n H qp [seed]. rewrite runFmap => H'.
-    suff : successful (run (@checker _ HCheck (pf x)) s seed) = true.
-    + subst.
-      remember (run (promote (props' n pf sh x)) s seed) as b. symmetry in Heqb.
-      rewrite runPromote in Heqb; subst. simpl.
-      case: n => [| n] /=;
-      by destruct ((run (checker (pf x)) s seed)) as [[res [l]]] => //=.
-      subst. apply H.
-      by eexists; eexists.
-Qed.
-
-Lemma semCover_id {C} `{Checkable C} (b: bool) (n: nat)
-                       (str : String.string) (c : C) (s : nat) :
-    semCheckerSize (cover b n str c) s <-> semCheckableSize c s.
-Proof.
-  split.
-  - rewrite /cover. case: b => //.
-    move => H1. apply mapTotalResult_id in H1 => //.
-      by move => [? ? ? ? ? ?].
-  - move => H1. rewrite /cover. case: b => //.
-    apply mapTotalResult_id => //.
-      by move => [? ? ? ? ? ?].
-Qed.
-
-Lemma semClassify_id {C} `{Checkable C} (b: bool) (str : String.string)
-          (c : C) (s : nat) :
-    semCheckerSize (classify b str c) s <-> semCheckableSize c s.
-Proof.
-  by rewrite /classify semCover_id.
-Qed.
-
-Lemma semLabel_id {C} `{Checkable C} (str : String.string) (c : C) (s : nat) :
-    semCheckerSize (label str c) s <-> semCheckableSize c s.
-Proof.
-  by rewrite /label semClassify_id.
-Qed.
-
-Lemma semCollect_id {C} `{Checkable C} (str : String.string) (c : C) (s : nat) :
-    semCheckerSize (collect str c) s <-> semCheckableSize c s.
-Proof.
-  by rewrite /collect semLabel_id.
-Qed.
-
-Open Scope Checker_scope.
-
-Lemma semImplicationSize {C} `{Checkable C} (c : C) (b : bool) s :
-  semCheckerSize (b ==> c) s <-> (b -> semCheckableSize c s).
-Proof.
-  case: b; split=> //=; first by move/(_ refl_equal).
-  by move=> ? ?; rewrite (semReturnSize _ _ _) => <-.
-Qed.
-
-(* equivalences for other combinators *)
-
-Lemma semReturnGen (qp : QProp) (s: nat) :
-    semCheckerSize (returnGen qp) s <-> semCheckableSize qp s.
-Proof.
-  rewrite /semChecker. split;
-  move => H qp' /semReturnSize Hprop; subst;
-  apply H; by apply semReturnSize.
-Qed.
-
-Lemma semBindGen {A} (gen : G A) (f : A -> Checker) (s: nat):
-    semCheckerSize (bindGen gen f) s <->
-    forall a, semGenSize gen s a -> semCheckerSize (f a) s.
-Proof.
-  unfold semCheckerSize. split.
-  - move => H a Hsize qp Hsize'. eapply H.
-    apply semBindSize.  eexists; split; eassumption.
-  - move => H qp /semBindSize [a [H1 H2]]. eapply H; eassumption.
-Qed.
-
-Lemma semPredQPropSize (c : Checker) (s : nat) :
-    semCheckableSize c s <-> (semCheckerSize c s).
-Proof.
-  rewrite /semCheckableSize /checker
-          /testChecker /checker /testProp /semCheckerSize.
-  split; move => Hqp qp Hsize; auto.
-Qed.
-
-(* begin semForAllSize *)
-Lemma semForAllSize {A C} `{Show A, Checkable C} (g : G A) (f : A -> C) (s:nat) :
-  semCheckerSize (forAll g f) s <->
-  forall (a : A), a \in semGenSize g s -> semCheckableSize (f a) s.
-(* end semForAllSize *)
-Proof.
-  split=> H'.
-  - rewrite /forAll in H'. move/semBindGen : H' => H' a /H' Hgen.
-      by apply semPrintTestCase_id in Hgen.
-  - rewrite /forAll in H' *. apply semBindGen => g' Hgen.
-    rewrite semPrintTestCase_id. by apply H'.
-Qed.
-
-(* CH: any way to relate this to generators and unsizedness of generators?
-   Yes, unsizedChecker should be defined in terms of unsized and semChecker' *)
-
-Definition genChecker c := fmap successful c.
-
-Definition unsizedChecker (c : Checker) : Prop := unsized (genChecker c).
-
-(* alternative definitions
-Definition unsizedChecker (c : Checker) : Prop :=
-  forall s1 s2, semCheckerSize c s1 <-> semCheckerSize c s2.
-
-(* another characterization of unsizedChecker *)
-Lemma unsizedChecker_def2 {A : Type} : forall (c : Checker),
-  unsizedChecker c ->
-  forall s, semCheckerSize c s <-> semChecker c.
-Proof.
-  intros. split; intro H'.
-  - intro s'. rewrite H. eassumption.
-  - by apply H'.
-Qed.
-*)
-
 Lemma imset_id' T (A : set T) f : (forall x, f x = x) -> f @: A <--> A.
 Proof.
   rewrite /imset /bigcup => H x. split.
   - move => [y [H1 H2]]. rewrite H in H2. inversion H2. subst. assumption.
   - move => H1. eexists. split. eassumption. by rewrite H.
-Qed.
-
-Lemma semMapTotalResult_id {C} `{Checkable C} f (c : C) :
-    (forall r, f r = r) ->
-    (semGen (mapTotalResult f c) <--> semGen (checker c)).
-Proof.
-  intros.
-  rewrite /mapTotalResult /mapRoseResult /mapProp.
-  rewrite semFmap. apply imset_id'. intros [?]. by rewrite fmapRose_id.
 Qed.
 
 Lemma another_one_for_maxime a b (f g : a -> b) (A : set a) :
@@ -288,51 +69,6 @@ Proof.
   rewrite /imset /bigcup /set1. move => H x.
   split => [[i [H1 H2]] | [i [H1 H2]]]; eexists; split;
            try eassumption. congruence. congruence.
-Qed.  
-
-Lemma semPrintTestCase_id' {C} `{Checkable C} (s: String.string) (c : C) :
-    successful @: semGen (printTestCase s c) <--> successful @: semGen (checker c).
-Proof.
-  intros. unfold printTestCase, callback.
-  rewrite /mapTotalResult /mapRoseResult /mapProp.
-  rewrite semFmap. rewrite -imset_comp. apply another_one_for_maxime.
-  simpl. move => [[[? ? ? ? ? ?] ?]]. reflexivity.
-Qed.
-
-(* CH: almost the same as before, should refactor at some point *)
-Lemma semPrintTestCase_id'' {C} `{Checkable C} (str : String.string) (c : C) s :
-    successful @: semGenSize (printTestCase str c) s <-->
-    successful @: semGenSize (checker c) s.
-Proof.
-  intros. unfold printTestCase, callback.
-  rewrite /mapTotalResult /mapRoseResult /mapProp.
-  rewrite semFmapSize. rewrite -imset_comp. apply another_one_for_maxime.
-  simpl. move => [[[? ? ? ? ? ?] ?]]. reflexivity.
-Qed.
-
-Lemma unsized_printTestCase {A C} `{Checkable C} `{Show A} (c : A -> C) :
-  (forall a, unsizedChecker (checker (c a))) ->
-  (forall a, unsizedChecker
-               (printTestCase (String.append (Show.show a) newline) (c a))).
-Proof.
-  rewrite /unsizedChecker /unsized /genChecker. setoid_rewrite semFmapSize.
-  move => H' a s1 s2. specialize (H' a s1 s2).
-  by do 2 rewrite semPrintTestCase_id''.
-Qed.
-
-(* This seems like a better way to prove semForAll *)
-Lemma semForAll_aux {A C} `{Show A, Checkable C} (g : G A) (f : A->C):
-  (forall a, unsizedChecker (checker (f a))) ->
-  successful @: semGen (forAll g f) <-->
-  (\bigcup_(a in semGen g) successful @: (semGen (checker (f a)))).
-Proof.
-  intros. rewrite /forAll.
-  rewrite -semFmap. rewrite semFmapBind.
-  rewrite semBindUnsized2.
-  apply eq_bigcupr => a.
-  rewrite semFmap.
-  apply semPrintTestCase_id'.
-  by apply unsized_printTestCase.
 Qed.
 
 Lemma subset_trans a (A1 A2 A3 : set a) :
@@ -350,56 +86,8 @@ Proof.
   rewrite /set_incl /bigcup. by eauto 3.
 Qed.
 
-(* CH: We could create a super class UCheckable that includes the
-       unsized assumption. And we could use sections to hide all the
-       type class stuff from the paper. *)
-(* CH: This will be affected by upcoming refactoring;
-       proving it like this only because it appears in ITP submission *)
-(* begin semForAll *)
-Lemma semForAll {A C:Type} `{Show A, Checkable C} (g : G A) (f : A->C) :
-    (forall a, unsizedChecker (checker (f a))) ->
-    (semChecker (forAll g f) <-> forall (a : A), semGen g a -> semCheckable (f a)).
-(* end semForAll *)
-Proof.
-  move=> uc.
-  rewrite /semCheckable semChecker_def3. setoid_rewrite semChecker_def3.
-  rewrite /genChecker.
-  split => H'.
-  - intros. move : H'. apply subset_trans.
-    rewrite semForAll_aux; [| by []].
-    by apply here_is_one_more with
-       (f:= fun x => successful @: semGen (checker (f x))).
-  - rewrite semForAll_aux; [| by []].
-    unfold set_incl in *. intros b [x [H1 H2]].
-    eapply H'; eassumption.
-Qed.
-
 Lemma subset_refl T (A : set T) : A \subset A.
 Proof. by rewrite /set_incl. Qed.
-
-(* begin semImplication *)
-Lemma semImplication {C} `{Checkable C} (b : bool) (c : C) :
-  semChecker (b ==> c) <-> (b -> semCheckable c).
-(* end semImplication *)
-Proof.
-  rewrite /semCheckable !semChecker_def3.
-  split => [H' b'|].
-  - by rewrite b' in H'.
-  - case b; simpl => H'. by apply H'.
-    rewrite semReturn /imset bigcup_set1. by apply subset_refl.
-Qed.
-
-Lemma semPredQPropNew:
-  forall (p : G QProp),
-    semCheckable p <-> (semChecker p).
-Proof. by rewrite /semCheckable /checker. Qed.
-
-
-Lemma bool_successful :  
-  forall b, resultSuccessful (liftBool b) = b.
-Proof.
-  intros. destruct b; auto.
-Qed.
 
 Lemma subset_singl : 
   forall {A} (x y : A), [set x] \subset [set y] <-> y = x. 
@@ -409,21 +97,447 @@ Proof.
   - apply subset_refl.
 Qed.
 
-(* begin semCheckableBool *)
-Lemma semCheckableBool (b : bool) : semCheckable b <-> b.
-(* end semCheckableBool *)
-Proof. 
-  (* CH: brute-force, please fix 
-     ZP : better now? We do case analysis on b bun in a lemma; 
-          I don't think we can avoid it *)
-  rewrite /semCheckable /checker semChecker_def3 /checker. simpl.
-  split; rewrite semReturn /imset bigcup_set1 /= bool_successful subset_singl;
-  now symmetry; auto. 
+(* End Lemmas for Maxime's library *) 
+
+
+(* another characterization of semChecker *)
+Lemma semChecker_def2 c :
+  semChecker c <-> (forall qp, semGen c qp -> successful qp = true).
+Proof.
+  rewrite /semChecker /semCheckerSize /semGen. split; intro H.
+  - intros. destruct H0 as [s [H0 Ho']]. symmetry; eapply (H s). eexists. 
+    split; eauto.  reflexivity.
+  - intros n b [qp [H1 H2]]. symmetry in H2. 
+    rewrite H2. symmetry. apply H.  
+    eexists; eauto. split; eauto. reflexivity.
 Qed.
 
-Definition uncurry {A B C : Type} (f : A * B -> C) (a : A) (b : B) := f (a,b).
+(* CH: This is the definition of Checker I would like to use *)
+(* ZP : For now semCheckerSize has a similar definition and 
+        semChecker is defined in terms of semCheckerSize *)
+Lemma semChecker_def3 c :
+  semChecker c <-> (successful @: semGen c \subset [set true]).
+Proof.
+  rewrite semChecker_def2. split; intro H.
+(*  CH: why can't I rewrite with semFmap directly? See tentative instances below *)
+  - intros b H'. unfold imset, bigcup in H'.
+    destruct H' as [qp [H1 H2]]. apply H in H1. by rewrite H1 in H2.
+  - intros. unfold set_incl in H. specialize (H (successful qp)).
+    unfold set1 in H. symmetry. apply H. clear H.
+    by apply one_more_for_maximes_library.
+Qed.
+
+
+(* What does it mean for checkers to be unsized/monotonic? *)
+
+(* CH: any way to relate this to generators and unsizedness of generators?
+   Yes, unsizedChecker should be defined in terms of unsized and semChecker' *)
+
+Definition genChecker c := fmap successful c.
+
+Definition unsizedChecker (c : Checker) : Prop := unsized (genChecker c).
+
+Definition sizeMonotonicChecker (c : Checker) : Prop := sizeMonotonic (genChecker c).
+
+Lemma unsizedCheckerDef (c : Checker) :
+  unsizedChecker c ->
+  forall s1 s2, semCheckerSize c s1 <-> semCheckerSize c s2.
+Proof.
+  rewrite /unsizedChecker /genChecker /unsized;
+  move => Hunsized s1 s2; rewrite /semCheckerSize; split;
+  move => H b [s [H1 <-]]; specialize (Hunsized s1 s2);
+  rewrite -> !semFmapSize in Hunsized;
+  apply H; apply Hunsized; exists s; split => //.
+Qed.
+
+Lemma sizeMonotonicCheckerDef (c : Checker) :
+  sizeMonotonicChecker c ->
+  forall s1 s2, s1 <= s2 -> semCheckerSize c s2 -> semCheckerSize c s1.
+Proof.
+  rewrite /sizeMonotonicChecker /sizeMonotonicChecker /sizeMonotonic /genChecker ;
+  move => Hmon s1 s2 Hle.
+  move => H b [s [H1 <-]]. specialize (Hmon s1 s2 Hle).
+  rewrite -> !semFmapSize in Hmon;
+  apply H; apply Hmon; exists s; split => //.
+Qed.
+
+Lemma unsizedCheckerWeak (c : Checker) :
+  unsized c ->
+  forall s1 s2, semCheckerSize c s1 <-> semCheckerSize c s2.
+Proof.
+  move => Hunsized s1 s2; rewrite /semCheckerSize; split;
+  move => H b [s [H1 <-]]; apply H; exists s; split => //;
+  eapply Hunsized; eauto. 
+Qed.
+
+Lemma sizeMonotonicCheckerWeak (c : Checker) :
+  sizeMonotonic c ->
+  forall s1 s2, s1 <= s2 -> semCheckerSize c s2 -> semCheckerSize c s1.
+Proof.
+  move => Hmon s1 s2 Hleq; rewrite /semCheckerSize.
+  move => H b [s [H1 <-]]. apply H; exists s; split => //.
+  eapply Hmon; eauto.
+Qed.
+
+Lemma mapTotalResult_idSize {C} `{Checkable C} (f : Result -> Result) (c : C) s :
+    (forall res, resultSuccessful res = resultSuccessful (f res)) ->
+    (semCheckerSize (mapTotalResult f c) s <-> semCheckableSize c s).
+Proof.
+  move=> eq_res. 
+  rewrite /mapTotalResult /mapRoseResult /mapProp/semCheckableSize /semCheckerSize. 
+  split; rewrite semFmapSize. 
+  - move => H1 b [[[res l]] /= [H2 H3]].
+    rewrite -H3 eq_res. apply H1.
+    repeat (eexists; split; eauto).
+  - move => /= H1 b [[[res l]] /= [[[[res' l'] [/= H2 [H3 H4]]] H5]]]; subst.
+    rewrite <- H5, <- eq_res in *.  apply H1.
+    eexists. split; eauto. reflexivity.
+Qed.
+
+Lemma mapTotalResult_id {C} `{Checkable C} (f : Result -> Result) (c : C) :
+    (forall res, resultSuccessful res = resultSuccessful (f res)) ->
+    (semChecker (mapTotalResult f c) <-> semCheckable c).
+Proof.
+  move=> eq_res; split => H' s; eapply mapTotalResult_idSize; eauto.
+  by apply H'.
+Qed.
+
+Lemma semCallback_idSize {C} `{Checkable C} (cb : Callback) (c : C) (s : nat) :
+    semCheckerSize (callback cb c) s <-> semCheckableSize c s.
+Proof.
+  rewrite /callback.
+  split; move => H'.
+  - apply mapTotalResult_idSize in H' => //;
+    by move => [? ? ? ? ? ?].
+  - apply mapTotalResult_idSize => //;
+    by move => [? ? ? ? ? ?].
+Qed.
+
+Lemma semCallback_id {C} `{Checkable C} (cb : Callback) (c : C) :
+    semChecker (callback cb c) <-> semCheckable c.
+Proof.
+  split => H' s; eapply semCallback_idSize; eauto.
+  by apply H'.
+Qed.
+
+Lemma semWhenFail_idSize {C} `{Checkable C} (str : String.string) (c : C) s :
+    semCheckerSize (whenFail str c) s <-> semCheckableSize c s.
+Proof.
+  by rewrite /whenFail semCallback_idSize.
+Qed.
+
+Lemma semWhenFail_id {C} `{Checkable C} (str : String.string) (c : C) :
+    semChecker (whenFail str c) <-> semCheckable c.
+Proof.
+  by rewrite /whenFail semCallback_id.
+Qed.
+
+Lemma semPrintTestCase_idSize {C} `{Checkable C} (str : String.string) (c : C) s :
+    semCheckerSize (printTestCase str c) s <-> semCheckableSize c s.
+Proof.
+  by rewrite /printTestCase semCallback_idSize.
+Qed.
+
+Lemma semPrintTestCase_id {C} `{Checkable C} (str : String.string) (c : C) :
+    semChecker (printTestCase str c) <-> semCheckable c.
+Proof.
+  by rewrite /printTestCase semCallback_id.
+Qed.
+
+Lemma semShrinking_idSize {C A} {HCheck : Checkable C}
+         (sh : A -> list A) (x : A) (pf : A -> C) (s : nat) :
+    semCheckerSize (shrinking sh x pf) s <->
+    semCheckableSize (pf x) s.
+Proof.
+  unfold semCheckableSize, shrinking, semCheckerSize, semGenSize, props.
+  have [n <-] : exists n, S n  = 1000 by eexists; reflexivity.
+  split.
+  - move => H b [[[res [l]]] [/= [seed Hgen] H']]; subst.
+    + suff :
+        successful
+          (run
+             (fmap
+                (fun x0 => {| unProp := joinRose (fmapRose unProp x0) |})
+                (promote (@props' _ _ HCheck (S n) pf sh x))) s seed).
+      setoid_rewrite runFmap. 
+      rewrite runPromote. simpl. rewrite Hgen -H' /=. 
+      move => -> //. 
+      rewrite <- H => //. eexists. split; try by reflexivity.
+      eexists. reflexivity.
+  - move => H b [[[r [l]]] /= [[seed H1] <-]]. apply H. 
+    rewrite runFmap runPromote /= in H1.
+    destruct ((run (checker (pf x)) s seed)) as [[res [l']]] eqn:Heq=> //=.
+    simpl in *. move : H1 => [H1 H2]; subst.
+    eexists. eexists. exists seed. reflexivity. rewrite Heq. reflexivity.
+Qed.
+    
+Lemma semShrinking_id {C A} {HCheck : Checkable C}
+         (sh : A -> list A) (x : A) (pf : A -> C)  :
+    semChecker (shrinking sh x pf) <->
+    semCheckable (pf x).
+Proof.
+  split; move => H s; eapply semShrinking_idSize; first by eauto.
+  by apply H.
+Qed.
+
+Lemma semCover_idSize {C} `{Checkable C} (b: bool) (n: nat)
+      (str : String.string) (c : C) (s : nat) :
+  semCheckerSize (cover b n str c) s <-> semCheckableSize c s.
+Proof.
+  split.
+  - rewrite /cover. case: b => //.
+    move => H1. apply mapTotalResult_idSize in H1 => //.
+      by move => [? ? ? ? ? ?].
+  - move => H1. rewrite /cover. case: b => //.
+    apply mapTotalResult_idSize => //.
+      by move => [? ? ? ? ? ?].
+Qed.
+
+Lemma semCover_id {C} `{Checkable C} (b: bool) (n: nat)
+      (str : String.string) (c : C) :
+  semChecker (cover b n str c) <-> semCheckable c.
+Proof.
+  split; move => H' s; eapply semCover_idSize; first by eauto.
+  by apply H'.
+Qed.
+
+Lemma semClassify_idSize {C} `{Checkable C} (b: bool) (str : String.string)
+          (c : C) (s : nat) :
+    semCheckerSize (classify b str c) s <-> semCheckableSize c s.
+Proof.
+  by rewrite /classify semCover_idSize.
+Qed.
+
+Lemma semClassify_id {C} `{Checkable C} (b: bool) (str : String.string) (c : C) :
+    semChecker (classify b str c) <-> semCheckable c.
+Proof.
+  by rewrite /classify semCover_id.
+Qed.
+
+Lemma semLabel_idSize {C} `{Checkable C} (str : String.string) (c : C) (s : nat) :
+    semCheckerSize (label str c) s <-> semCheckableSize c s.
+Proof.
+  by rewrite /label semClassify_idSize.
+Qed.
+
+Lemma semLabel_id {C} `{Checkable C} (str : String.string) (c : C) :
+    semChecker (label str c) <-> semCheckable c.
+Proof.
+  by rewrite /label semClassify_id.
+Qed.
+
+Lemma semCollect_idSize {C} `{Checkable C} (str : String.string) (c : C) (s : nat) :
+    semCheckerSize (collect str c) s <-> semCheckableSize c s.
+Proof.
+  by rewrite /collect semLabel_idSize.
+Qed.
+
+Lemma semCollect_id {C} `{Checkable C} (str : String.string) (c : C) :
+    semChecker (collect str c) <-> semCheckable c.
+Proof.
+  by rewrite /collect semLabel_id.
+Qed.
+
+Open Scope Checker_scope.
+
+Lemma semImplicationSize {C} `{Checkable C} (c : C) (b : bool) s :
+  semCheckerSize (b ==> c) s <-> (b -> semCheckableSize c s).
+Proof.
+  case: b; split=> //=; first by move/(_ refl_equal).
+  by move => _ b [x [/semReturnSize <- <-]].
+Qed.
+
+(* begin semImplication *)
+Lemma semImplication {C} `{Checkable C} (c : C) (b : bool) :
+  semChecker (b ==> c) <-> (b -> semCheckable c).
+(* end semImplication *)
+Proof.
+  split; [move => H1 b' s' | move => H1 s b'];
+  eapply semImplicationSize; try by eauto.
+  move => b''. by apply H1.
+Qed.
+
+(* equivalences for other combinators *)
+
+Lemma semReturnGenSize (qp : QProp) (s: nat) :
+    semCheckerSize (returnGen qp) s <-> semCheckableSize qp s.
+Proof.
+  rewrite /semCheckerSize. split.
+  - move =>  H qp' [x [H1 H2]]. apply H. eexists; split; eauto. 
+  - move => H b [x [H1 H2]] //. apply H => //=. eexists; split; eauto.
+Qed.
+
+Lemma semReturnGen (qp : QProp) :
+    semChecker (returnGen qp) <-> semCheckable qp.
+Proof. 
+  split; move => H s.
+  - by move /(_ s) /semReturnGenSize : H => //. 
+  - apply semReturnGenSize; eauto. by apply H.
+Qed.
+
+Lemma semBindGenSize {A} (gen : G A) (f : A -> Checker) (s: nat):
+    semCheckerSize (bindGen gen f) s <->
+    forall a, semGenSize gen s a -> semCheckerSize (f a) s.
+Proof.
+  unfold semCheckerSize. split.
+  - move => H a Hsize b [qp [H1 <-]]. apply H.
+    exists qp; split => //=. apply semBindSize. eexists; split; eauto.
+  - move => H b [qp [/semBindSize [a [H1 H2]] <-]]. eapply H; try eassumption.
+    eexists; split => //; eauto.
+Qed.
+
+Lemma semBindGenUsinzed1 {A} (gen : G A) (f : A -> Checker) :
+    unsized gen ->
+    (semChecker (bindGen gen f) <->
+     forall a, semGen gen a -> semChecker (f a)).
+Proof.
+  move => Hunsized. split; move => H a.
+  - move => [s [_ H']] s'. eapply Hunsized in H'.
+    by eapply semBindGenSize in H; eauto.
+  - by eapply semBindGenSize; intros; apply H; eexists; split => //; eauto.
+Qed.
+
+Lemma semBindGenUsinzed2 {A} (gen : G A) (f : A -> Checker) :
+    (forall a, unsizedChecker (f a)) ->
+    (semChecker (bindGen gen f) <->
+     forall a, semGen gen a -> semChecker (f a)).
+Proof.
+  move => Hunsized. split; move => H a.
+  - move => [s [_ H']] s'.
+    eapply semBindGenSize in H; last by eauto.
+    eapply unsizedCheckerDef; eauto.
+  - by eapply semBindGenSize; intros; apply H; eexists; split => //; eauto.
+Qed.
+
+Lemma semBindGenSizeMonotonic {A} (gen : G A) (f : A -> Checker) :
+  sizeMonotonic gen ->  
+  (forall a, sizeMonotonicChecker (f a)) ->
+  (semChecker (bindGen gen f) <->
+   forall a, semGen gen a -> semChecker (f a)).
+Proof.
+  move => Hmon1 Hmon2. split; move => H a.
+  - move => [s [_ H']] s'. case_eq (s <= s') => [Hleq |  
+                                                 /leP/Compare_dec.not_le/ltP/ltnW Hleq].
+    + specialize (H s').
+      eapply semBindGenSize in H; eauto. eapply Hmon1; eauto.
+    + specialize (H s). eapply semBindGenSize in H; eauto. 
+      eapply sizeMonotonicCheckerDef; eauto. 
+  - by eapply semBindGenSize; intros; apply H; eexists; split => //; eauto.
+Qed.
+
+
+Lemma semPredQPropSize (c : Checker) (s : nat) :
+    semCheckableSize c s <-> (semCheckerSize c s).
+Proof.
+  rewrite /semCheckableSize /checker
+          /testChecker /checker /testProp /semCheckerSize.
+  split; move => Hqp qp Hsize; auto.
+Qed.
+
+Lemma semPredQProp (c : Checker) :
+    semCheckable c <-> semChecker c.
+Proof.
+  split => H s; eapply semPredQPropSize; eauto.
+Qed.
+
+(* begin semForAllSize *)
+Lemma semForAllSize {A C} `{Show A, Checkable C} (g : G A) (f : A -> C) (s:nat) :
+  semCheckerSize (forAll g f) s <->
+  forall (a : A), a \in semGenSize g s -> semCheckableSize (f a) s.
+(* end semForAllSize *)
+Proof.
+  split=> H'.
+  - rewrite /forAll in H'. move/semBindGenSize : H' => H' a /H' Hgen.
+      by apply semPrintTestCase_idSize in Hgen.
+  - rewrite /forAll in H' *. apply semBindGenSize => g' Hgen.
+    rewrite semPrintTestCase_idSize. by apply H'.
+Qed.
+
+Lemma semForAllUnsized1 {A C} `{Show A, Checkable C} (g : G A) (f : A -> C) :
+  unsized g ->
+  (semChecker (forAll g f) <->
+   forall (a : A), a \in semGen g -> semCheckable (f a)).
+Proof.
+  split=> H'.
+  - move => a [s' [_ Hgen]] s. specialize (H' s).
+    eapply semForAllSize in H'; first by eauto.
+    eapply H1; eauto.
+  - move => s; eapply semForAllSize; move => a Hgen. 
+    apply H'; eexists; split => //; eauto. 
+Qed.
+
+(* begin semForAll *)
+Lemma semForAllUnsized2 {A C} `{Show A, Checkable C} (g : G A) (f : A -> C) :
+  (forall a, unsizedChecker (checker (f a))) ->
+  (semChecker (forAll g f) <->
+   forall (a : A), a \in semGen g -> semCheckable (f a)).
+(* end semForAll *)
+Proof.
+  split=> H'.
+  - move => a [s' [_ Hgen]] s. specialize (H' s').
+    eapply semForAllSize in H'; last by eauto.
+    eapply unsizedCheckerDef; eauto.
+  - move => s; eapply semForAllSize; move => a Hgen. 
+    apply H'; eexists; split => //; eauto. 
+Qed.
+
+Lemma semForAllSizeMonotonic {A C} `{Show A, Checkable C} (g : G A) (f : A -> C) :
+  sizeMonotonic g ->
+  (forall a, sizeMonotonicChecker (checker (f a))) ->
+  (semChecker (forAll g f) <->
+   forall (a : A), a \in semGen g -> semCheckable (f a)).
+Proof.
+  move => Hmon1 Hmon2. split; move => Hcheck a.
+  - move => [s [_ H']] s'. case_eq (s <= s') => [Hleq |  
+                                                 /leP/Compare_dec.not_le/ltP/ltnW Hleq].
+    + specialize (Hcheck s').
+      rewrite -> semForAllSize in Hcheck. apply Hcheck. 
+      by eapply Hmon1; eauto.
+    + specialize (Hcheck s). eapply semForAllSize in Hcheck; eauto. 
+      by eapply sizeMonotonicCheckerDef; eauto. 
+  - by eapply semForAllSize; intros; apply Hcheck; eexists; split => //; eauto.
+Qed.
+
+
+Lemma unsized_printTestCase {A C} `{Checkable C} `{Show A} (c : A -> C) :
+  (forall a, unsized (checker (c a))) ->
+  (forall a, unsized (printTestCase (String.append (Show.show a) newline) (c a))).
+Proof.
+(*   rewrite /unsizedChecker /unsized. setoid_rewrite semFmapSize. *)
+(*   move => H' a s1 s2. specialize (H' a s1 s2). *)
+(*   by do 2 rewrite semPrintTestCase_idSize. *)
+(* Qed. *)
+Abort.
+
+
+
+
+(* alternative definitions
+Definition unsizedChecker (c : Checker) : Prop :=
+  forall s1 s2, semCheckerSize c s1 <-> semCheckerSize c s2.
+
+(* another characterization of unsizedChecker *)
+Lemma unsizedChecker_def2 {A : Type} : forall (c : Checker),
+  unsizedChecker c ->
+  forall s, semCheckerSize c s <-> semChecker c.
+Proof.
+  intros. split; intro H'.
+  - intro s'. rewrite H. eassumption.
+  - by apply H'.
+Qed.
+*)
+
+(* CH: We could create a super class UCheckable that includes the
+       unsized assumption. And we could use sections to hide all the
+       type class stuff from the paper. *)
+(* CH: This will be affected by upcoming refactoring;
+       proving it like this only because it appears in ITP submission *)
+
+
 
 Require Import FunctionalExtensionality.
+
+Definition uncurry {A B C : Type} (f : A * B -> C) (a : A) (b : B) := f (a,b).
 
 Lemma curry_uncurry {A B C : Type} (f : A * B -> C) :
   curry (uncurry f) = f.
@@ -442,117 +556,181 @@ Proof. move => a b H. by rewrite H. Qed.
    semBindSizeMonotonic instead of semBindUnsized2?  *)
 (* CH: The problem with proving this is the silly print in the middle of things.
    There are also some technical problems with setoid_rewriting taking ages,
-   and requiring an useless split beforehand. *)
+   and requiring an useless split beforehand. 
+   ZP: Got rid of setoid_rewrite. The proof goes through instantly now.   
+*)
 Lemma mergeForAlls {A B C : Type} `{Checkable C} `{Show A} `{Show B}
          (ga : G A) (gb : G B) (f : A -> B -> C) :
      semChecker (forAll ga (fun a => forAll gb (f a))) <->
      semChecker (forAll (genPair ga gb) (curry f)).
 Proof.
-  rewrite /forAll.
-  do 2 rewrite semChecker_def3.
-  rewrite /semGen.
-  split. (* this is a very silly split only to make rewriting work *)
-  - setoid_rewrite semBindSize.
-    repeat setoid_rewrite imset_bigcup.
-    setoid_rewrite semPrintTestCase_id''. simpl.
-    setoid_rewrite semBindSize.
-    setoid_rewrite imset_bigcup.
-    setoid_rewrite semPrintTestCase_id''.
-    repeat setoid_rewrite <- imset_bigcup.
-    repeat setoid_rewrite <- semBindSize.
-(* for some reason this match doesn't work
-    match goal with
-    | [ |- context[ (\bigcup_(x in [set: nat]) semGenSize ?G x) ]] =>
-      fold (bindGen G x)
-    end.
-*)
-    fold (semGen (bindGen ga
-            (fun a : A => bindGen gb (fun a0 : B => checker (f a a0))))).
-    fold (semGen
-         (bindGen (genPair ga gb) (fun a : A * B => checker (curry f a)))).
-    rewrite mergeBinds. apply eq_to_impl. repeat f_equal.
-    apply functional_extensionality. move => [a b]. reflexivity.
-  - (* copy paste from above, we clearly shouldn't split here! *)
-  - setoid_rewrite semBindSize.
-    repeat setoid_rewrite imset_bigcup.
-    setoid_rewrite semPrintTestCase_id''. simpl.
-    setoid_rewrite semBindSize.
-    setoid_rewrite imset_bigcup.
-    setoid_rewrite semPrintTestCase_id''.
-    repeat setoid_rewrite <- imset_bigcup.
-    repeat setoid_rewrite <- semBindSize.
-    fold (semGen (bindGen ga
-            (fun a : A => bindGen gb (fun a0 : B => checker (f a a0))))).
-    fold (semGen
-         (bindGen (genPair ga gb) (fun a : A * B => checker (curry f a)))).
-    rewrite mergeBinds. apply eq_to_impl. repeat f_equal.
-    apply functional_extensionality. move => [a b]. reflexivity.
+  (* ZP : I know that this proof lacks nice point-free reasoning, but it is 
+          significantly smaller and typechecks much faster that the previous one *)
+  split. 
+  - move => HforAll s. apply semForAllSize; 
+    move  => [a b] /= /semLiftGen2Size [[a' b'] [[/= Hg1 Hg2] [Heq1 Heq2]]]; subst.
+    specialize (HforAll s). eapply semForAllSize in HforAll.
+    by eapply semForAllSize in HforAll; eauto. by eauto.
+  - move => HforAll s. apply semForAllSize => a Hgena. 
+    apply semForAllSize => b Hgenb.
+    specialize (HforAll s). 
+    move /semForAllSize/(_ (a, b)) : HforAll => /= HforAll. apply HforAll.
+    apply semLiftGen2Size. exists (a, b); split => //; eauto.
 Qed.
 
-Lemma semForAllShrink:
+Lemma semForAllShrinkSize:
   forall {A C} `{Checkable C} `{Show A}
          (gen : G A) (f : A -> C) shrinker (size: nat),
     semCheckerSize (forAllShrink gen shrinker f) size <->
     forall a : A, semGenSize gen size a -> semCheckableSize (f a) size.
 Proof.
   move => A C H show gen pf shrink. split.
-  - rewrite /forAllShrink semBindGen.
-    move=> H' a /H' Hgen. setoid_rewrite semShrinking_id in Hgen.
+  - rewrite /forAllShrink semBindGenSize.
+    move=> H' a /H' Hgen. setoid_rewrite semShrinking_idSize in Hgen.
     setoid_rewrite semPredQPropSize in Hgen.
-    by apply semPrintTestCase_id in Hgen.
-  - move=> H'. rewrite /forAllShrink semBindGen. move => a g.
-    rewrite semShrinking_id. apply semPredQPropSize.
-    rewrite semPrintTestCase_id. by auto.
+    by apply semPrintTestCase_idSize in Hgen.
+  - move=> H'. rewrite /forAllShrink semBindGenSize. move => a g.
+    rewrite semShrinking_idSize. apply semPredQPropSize.
+    rewrite semPrintTestCase_idSize. by auto.
 Qed.
 
-
-(* equivalent Props for Checkables *)
-
-Lemma semBool (b : bool) size : semCheckableSize b size <-> b.
+Lemma semForAllShrinkUnsized1 :
+  forall {A C} `{Checkable C} `{Show A}
+         (gen : G A) (f : A -> C) shrinker,
+    unsized gen ->
+    (semChecker (forAllShrink gen shrinker f) <->
+     forall a : A, semGen gen a -> semCheckable (f a)).
 Proof.
-case: b; split=> //.
-  by move=> _ ?; rewrite (semReturnSize _ _ _)  => <-.
-move=> /(_ (MkProp (MkRose (liftBool false) (lazy nil)))).
-by apply; rewrite (semReturnSize _ _ _).
+  split=> H'.
+  - move => a [s' [_ Hgen]] s. specialize (H' s).
+    eapply semForAllShrinkSize in H'; first by eauto.
+    eapply H1; eauto.
+  - move => s; eapply semForAllShrinkSize; move => a Hgen. 
+    apply H'; eexists; split => //; eauto. 
 Qed.
 
-Lemma semResult:
+Lemma semForAllShrinkUnsized2 :
+  forall {A C} `{Checkable C} `{Show A}
+         (gen : G A) (f : A -> C) shrinker,
+  (forall a, unsizedChecker (checker (f a))) ->
+  (semChecker (forAllShrink gen shrinker f) <->
+     forall a : A, semGen gen a -> semCheckable (f a)).
+Proof.
+  split=> H'.
+  - move => a [s' [_ Hgen]] s. specialize (H' s').
+    eapply semForAllShrinkSize in H'; last by eauto.
+    eapply unsizedCheckerDef; eauto.
+  - move => s; eapply semForAllShrinkSize; move => a Hgen. 
+    apply H'; eexists; split => //; eauto. 
+Qed.
+
+Lemma semForAllShrinkMonotonic :
+  forall {A C} `{Checkable C} `{Show A}
+         (gen : G A) (f : A -> C) shrinker,
+  sizeMonotonic gen ->
+  (forall a, sizeMonotonicChecker (checker (f a))) ->
+  (semChecker (forAllShrink gen shrinker f) <->
+     forall a : A, semGen gen a -> semCheckable (f a)).
+Proof.
+  move => A C H1 H2 gen f sh Hmon1 Hmon2. 
+  split; move => Hcheck a.
+  - move => [s [_ H']] s'. case_eq (s <= s') => [Hleq |  
+                                                 /leP/Compare_dec.not_le/ltP/ltnW Hleq].
+    + specialize (Hcheck s').
+      rewrite -> semForAllShrinkSize in Hcheck. apply Hcheck. 
+      by eapply Hmon1; eauto.
+    + specialize (Hcheck s). eapply semForAllShrinkSize in Hcheck; eauto. 
+      by eapply sizeMonotonicCheckerDef; eauto. 
+  - by eapply semForAllShrinkSize; intros; apply Hcheck; eexists; split => //; eauto.
+Qed.
+
+Lemma bool_successful :  
+  forall b, resultSuccessful (liftBool b) = b.
+Proof.
+  intros. destruct b; auto.
+Qed.
+
+Lemma semCheckableBoolSize (b : bool) size : semCheckableSize b size <-> b.
+Proof.
+  rewrite /semCheckableSize /semCheckerSize /checker /testBool.
+  split.
+  - move => /(_ b) H. 
+    suff : [set true] b by move => <- //.
+    eapply H. eexists (MkProp (MkRose (liftBool b) (lazy nil))).
+    split => //=. by rewrite -> (semReturnSize _ _ _). by eapply bool_successful.
+  - move => Hb b' [qp [/semReturnSize <- <-]] /=.
+    by rewrite bool_successful. 
+Qed.
+
+(* begin semCheckableBool *)
+Lemma semCheckableBool (b : bool) : semCheckable b <-> b.
+(* end semCheckableBool *)
+Proof. 
+  (* CH: brute-force, please fix 
+     ZP : better now? We do case analysis on b bun in a lemma; 
+          I don't think we can avoid it *)
+  split; [move => /(_ 0) H | move => H s]; eapply semCheckableBoolSize; eauto.
+Qed.
+ 
+Lemma semCheckableResultSize:
   forall (res: Result) (size: nat),
     semCheckableSize res size <-> resultSuccessful res.
 Proof.
-  rewrite /semCheckableSize /checker /testResult /semCheckerSize.
-  move => res. split.
-  + move=> /(_ ({| unProp := returnRose res |})) /= H.
-    apply H. by apply semReturnSize.
-  + by move=> H [[res' l]] /semReturnSize [Heq2 Heq3]; subst.
+  rewrite /semCheckableSize /checker /testResult /=.
+  move => res size. split. 
+  - move => /(_ (resultSuccessful res)) H. 
+    suff : [set true] (resultSuccessful res) by move <-.
+    apply H. eexists. split; first by apply semReturnSize. 
+    reflexivity. 
+  - move => H b [qp' [/semReturnSize <- <-]] //=.
 Qed.
 
-Lemma semUnit (t : unit) size : semCheckableSize t size <-> True.
+Lemma semCheckableResult :
+  forall (res: Result),
+    semCheckable res  <-> resultSuccessful res.
 Proof.
-by split=> // _ qp /semReturnSize <-.
+  split; [move => /(_ 0) H | move => H s]; eapply semCheckableResultSize; eauto.
 Qed.
 
-Lemma semQProp (qp : QProp) size :
+Lemma semCheckableUnitSize (t : unit) size : semCheckableSize t size <-> True.
+Proof.
+  split => // _ qp [qp' [/semReturnSize <- <-]] //.
+Qed.
+
+Lemma semCheckableUnit (t : unit) : semCheckable t <-> True.
+Proof.
+  split; [move => /(_ 0) H | move => H s]; eapply semCheckableUnitSize; eauto.
+Qed.
+
+Lemma semCheckableQPropSize (qp : QProp) size :
   semCheckableSize qp size <-> successful qp.
 Proof.
-by split=> [|? qp' /semReturnSize <-] //; apply; apply/semReturnSize.
+  rewrite /semCheckableSize /checker /testProp.
+  split. 
+  - move => /(_ (successful qp)) H. 
+    suff : ([set true] (successful qp)) by move => <-.
+    apply H. eexists. split ; last by reflexivity.
+    by apply semReturnSize.
+  - move => H b [qp' [/semReturnSize <- <-]] //=.
 Qed.
 
-Lemma semGen:
+Lemma semCheckableQProp (qp : QProp) :
+  semCheckable qp  <-> successful qp.
+Proof.
+  split; [move => /(_ 0) H | move => H s]; eapply semCheckableQPropSize; eauto.
+Qed.
+
+Lemma semCheckableGenSize:
   forall (P : Type) {H : Checkable P} (gen: G P) (size : nat),
     (semCheckableSize gen size) <->
     (forall p, semGenSize gen size p -> semCheckableSize p size).
 Proof.
-  move=> P H gen. unfold semCheckableSize, semCheckerSize in *. split.
-  - move=> Hsem qp Hsize.
-    move => qp' Hprop. simpl in *.
-    apply Hsem. apply semBindSize. exists qp.
-    by split => //.
-  - move => Hsem qp /semBindSize [p [Hsize Hsize']].
-    eapply Hsem; eassumption.
+  move=> P H gen s. rewrite /semCheckableSize /checker /testGenProp. split.
+  - move => /semBindGenSize Hcheck p Hgen //=; eauto.
+  - move => Hcheck. apply semBindGenSize => a Hgen; eauto.
 Qed.
 
-Lemma semFun:
+Lemma semCheckableFunSize:
   forall {A C} {H1 : Show A} {H2 : Arbitrary A} {H3 : Checkable C}
          (f : A -> C) (size: nat),
     semCheckableSize f size <->
@@ -561,25 +739,25 @@ Proof.
   move=> A C H1 H2 H3 f.
   rewrite /semCheckable /checker /testFun.
   split.
-  - move => /semForAllShrink H' a' /H' Gen. by auto.
-  - move => H'. apply semForAllShrink => a' /H' Hgen. by auto.
+  - move => /semForAllShrinkSize H' a' /H' Gen. by auto.
+  - move => H'. apply semForAllShrinkSize => a' /H' Hgen. by auto.
 Qed.
 
-Lemma semPolyFun:
+Lemma semCheckablePolyFunSize:
   forall {C : Type -> Type} {H : Checkable (C nat)} (f : forall T, C T)
          (size : nat),
     (semCheckableSize f size) <-> (semCheckableSize (f nat) size).
 Proof.
   move => C H f s. rewrite /semCheckableSize {2}/checker /testPolyFun.
-  by rewrite semPrintTestCase_id.
+  by rewrite semPrintTestCase_idSize.
 Qed.
 
-Lemma semPolyFunSet:
+Lemma semCheckablePolyFunSetSize:
   forall {C : Set -> Type} {H : Checkable (C nat)} (f : forall T, C T) (size: nat),
     (semCheckableSize f size) <->  (semCheckableSize (f nat) size).
 Proof.
   move => C H f s. rewrite /semCheckableSize {2}/checker /testPolyFun.
-  by rewrite semPrintTestCase_id.
+  by rewrite semPrintTestCase_idSize.
 Qed.
 
 (* A typeclass so we can automate the application of the previous theorems
@@ -596,7 +774,7 @@ Program Instance proveResult : Provable Result :=
     proposition s r := resultSuccessful r
   |}.
 Next Obligation.
-  by rewrite semResult.
+  by rewrite semCheckableResultSize.
 Qed.
 
 Program Instance proveUnit : Provable unit :=
@@ -604,7 +782,7 @@ Program Instance proveUnit : Provable unit :=
     proposition := fun _ _ => True
   |}.
 Next Obligation.
-  by rewrite semUnit.
+  by rewrite semCheckableUnitSize.
 Qed.
 
 Program Instance proveQProp : Provable QProp :=
@@ -612,7 +790,7 @@ Program Instance proveQProp : Provable QProp :=
     proposition s qp := successful qp = true
   |}.
 Next Obligation.
-  by rewrite semQProp.
+  by rewrite semCheckableQPropSize.
 Qed.
 
 Program Instance proveBool : Provable bool :=
@@ -620,7 +798,7 @@ Program Instance proveBool : Provable bool :=
     proposition s b :=  b = true
   |}.
 Next Obligation.
-  by rewrite semBool.
+  by rewrite semCheckableBoolSize.
 Qed.
 
 Program Instance proveGenProp {C} `{Provable C} :
@@ -630,8 +808,8 @@ Program Instance proveGenProp {C} `{Provable C} :
   |}.
 Next Obligation.
   destruct H0 as [semP proof]. rewrite /proposition. split.
-  - move => H'. apply semGen=> p Hgen. apply proof. eapply H'. eassumption.
-  - move => /semGen H' p Hgen. eapply proof. apply H'. by auto.
+  - move => H'. apply semCheckableGenSize => p Hgen. apply proof. eapply H'. eassumption.
+  - move => /semCheckableGenSize H' p Hgen. eapply proof. apply H'. by auto.
 Qed.
 
 Program Instance proveChecker : Provable Checker :=
@@ -652,9 +830,9 @@ Program Instance proveFun {A C: Type} `{Arbitrary A} `{Show A}
   |}.
 Next Obligation.
   destruct H2 as [semP proof]. rewrite /proposition. split.
-  - move=> H'. apply semFun => a' /H' Hgen.
+  - move=> H'. apply semCheckableFunSize => a' /H' Hgen.
     by apply proof.
-  - move=> H' a' Hgen. apply proof. by apply semFun.
+  - move=> H' a' Hgen. apply proof. by apply semCheckableFunSize.
 Qed.
 
 Program Instance provePolyFun {C : Type -> Type} `{Provable (C nat)} :
@@ -664,8 +842,8 @@ Program Instance provePolyFun {C : Type -> Type} `{Provable (C nat)} :
   }.
 Next Obligation.
   destruct H0 as [semP proof]. rewrite /proposition. split.
-  - move=> /proof H'. by apply semPolyFun.
-  - move=> /semPolyFun H'. by apply proof.
+  - move=> /proof H'. by apply semCheckablePolyFunSize.
+  - move=> /semCheckablePolyFunSize H'. by apply proof.
 Qed.
 
 Program Instance provePolyFunSet {C : Set -> Type} `{Provable (C nat)} :
@@ -675,6 +853,6 @@ Program Instance provePolyFunSet {C : Set -> Type} `{Provable (C nat)} :
   }.
 Next Obligation.
   destruct H0 as [semP proof]. rewrite /proposition. split.
-  - move=> /proof H'. by apply semPolyFunSet.
-  - move=> /semPolyFunSet H'. by apply proof.
+  - move=> /proof H'. by apply semCheckablePolyFunSetSize.
+  - move=> /semCheckablePolyFunSetSize H'. by apply proof.
 Qed.
